rt haskell+design+proof: reduce use of active_sc_at' in CRefine
This is achieved by asserting active_sc_at' in the appropriate
places within the Haskell.

Signed-off-by: Michael McInerney <michael.mcinerney@proofcraft.systems>

spec/haskell/src/SEL4/Model/StateData.lhs
@@ -533,6 +533,11 @@ An assert that will say that there is a scheduling context at the given pointer
 > sc_at'_asrt :: PPtr SchedContext -> KernelState -> Bool
 > sc_at'_asrt _ _ = True
 
+An assert that will say that there is an active scheduling context at the given pointer
+
+> active_sc_at'_asrt :: PPtr SchedContext -> KernelState -> Bool
+> active_sc_at'_asrt _ _ = True
+
 An assert that will say that valid_tcbs' holds
 
 > valid_tcbs'_asrt :: KernelState -> Bool
